\documentclass{article}
\usepackage[T1,T2A]{fontenc}
\usepackage[utf8]{inputenc}
\usepackage[english,russian]{babel}
\usepackage{xcolor}
\usepackage{amsmath}
\usepackage{amsfonts,bm}
\usepackage{tikz}
\usetikzlibrary{patterns}
\usetikzlibrary{quotes,angles}
\usepackage{relsize}

\title{Решение Задачи №34}
\author{Серёжи Фуканчика\\34 Ю класс}
\date{Январь 2020}

\begin{document}

\maketitle

\section{Задача}
Замена переменных
$$
\frac{1}{x^2}-\frac{1}{(x+1)^2}=1
$$

\section{Решение}
Возвратное.
$$
\frac{1}{x^2}-\frac{1}{(x+1)^2}=1
$$

$$
\frac{(x+1)^2}{x^2\cdot{}(x+1)^2}-\frac{x^2}{x^2\cdot{}(x+1)^2}-1=0
$$

$$
\frac{(x+1)^2-x^2}{x^2\cdot{}(x+1)^2}-1=0
$$

$$
\frac{(x+1)^2-x^2}{x^2\cdot{}(x+1)^2}-\frac{x^2\cdot{}(x+1)^2}{x^2\cdot{}(x+1)^2}=0
$$

$$
\frac{(x+1)^2-x^2-x^2\cdot{}(x+1)^2}{x^2\cdot{}(x+1)^2}=0
$$

$$
\frac{x^2+2x+1-x^2-x^2\cdot{}(x+1)^2}{x^2\cdot{}(x+1)^2}=0
$$

$$
\frac{2x+1-x^2\cdot{}(x+1)^2}{x^2\cdot{}(x+1)^2}=0
$$

$$
\frac{2x+1-x^2\cdot{}(x+1)^2}{x^2\cdot{}(x+1)^2}=0
$$

$$
\frac{2x+1-x^2\cdot{}(x^2+2x+1)}{x^2\cdot{}(x+1)^2}=0
$$

$$
\frac{2x+1-(x^4+2x^3+x^2)}{x^2\cdot{}(x+1)^2}=0
$$

$$
\frac{x^4+2x^3+x^2-2x-1}{x^2\cdot{}(x+1)^2}=0
$$

$$
\frac{x^4+2x^3+x^2-2x-1}{x^2\cdot{}(x+1)^2}=0
$$

$$
\frac{x^4-1+x^2+2x^3-2x}{x^2\cdot{}(x+1)^2}=0
$$

$$
\frac{\left(x^2-\frac{1}{x^2}\right)+1+2x-\frac{2}{x}}{x^2\cdot{}(x+1)^2}=0
$$

$$
\frac{\left(x^2-\frac{1}{x^2}\right)+1+2\left(x-\frac{1}{x}\right)}{x^2\cdot{}(x+1)^2}=0
$$

$$(x-\frac{1}{x})^2=x^2-2\cdot{}x\cdot{}\frac{1}{x}+\frac{1}{x^2}=x^2+\frac{1}{x^2}-2$$
\section{Ответ}

\section{Проверка}

\end{document}
% https://www.youtube.com/watch?v=oPVu1xafLkk
% https://www.youtube.com/watch?v=CDx0YlNs_E0
% https://www.youtube.com/watch?v=zg5rrRgI2AM

